concurrency/framework/AIO.s.dfy
@@ -105,6 +105,14 @@ abstract module AIO(aioparams: AIOParams, ioifc: InputOutputIfc, ssm: DiskSSM(io
       g: aioparams.WriteG)
   }
 
+  method {:extern} init_ctx(
+      ghost async_read_inv: (Ptr, Iocb, PointsToArray<byte>, aioparams.ReadG) -> bool,
+      ghost async_write_inv: (Ptr, Iocb, seq<byte>, aioparams.WriteG) -> bool
+    )
+  returns (linear ioctx: IOCtx)
+  ensures ioctx.async_read_inv == async_read_inv
+  ensures ioctx.async_write_inv == async_write_inv
+
   method {:extern} async_write(
       shared ctx: IOCtx,
       iocb_ptr: Ptr,
